generalize wp for strong/weak

PcolIris/Logic/WeakestPre.lean
@@ -7,9 +7,11 @@ import PcolIris.OProp.OProp
 
 namespace Pcol
 
-def wp (𝓘 : Inv) (c : Cmd Act) (ψ : OProp) : OProp :=
+def wp_base (𝓘 : Inv) (F : ProbSpace → Prop) (c : Cmd Act) (ψ : OProp) : OProp :=
   fun 𝓟 ↦
     ∀ (μ : Distr Mem) (𝓟fr : ProbSpace),
+      -- The frame validity predicate holds
+      F 𝓟fr →
       -- The initial distribution `μ` is a refinement of the precondition
       -- `𝓟`, the frame `𝓟fr`, and the invariant `𝓘`
       ((𝓟 ⊗ 𝓟fr ⊗ ProbSpace.trivial 𝓘.to_MProp) ≼ μ) →
@@ -18,18 +20,26 @@ def wp (𝓘 : Inv) (c : Cmd Act) (ψ : OProp) : OProp :=
       -- Then `ν` refines some probability space `𝓠`, which satisfies the postcondition `ψ`
         ∃ 𝓠, ((𝓠 ⊗ 𝓟fr ⊗ ProbSpace.trivial 𝓘.to_MProp) ≼ ν) ∧ ψ 𝓠
 
+/-- The standard "strong" wp allows any frame -/
+def wp (𝓘 : Inv) : Cmd Act → OProp → OProp := wp_base 𝓘 (fun _ ↦ True)
+
+/-- The "weak" triple only preserves frames for trivial probability spaces,
+where every event has probability exactly 0 or 1 -/
+def wp_weak (𝓘 : Inv) : Cmd Act → OProp → OProp := wp_base 𝓘 fun 𝓟fr ↦
+  ∀ E, 𝓟fr.mspace.MeasurableSet' E → 𝓟fr.μ E = 0 ∨ 𝓟fr.μ E = 1
+
 notation 𝓘 " ⊢{{" φ "}} " c " {{" ψ "}}" => φ ⊢ wp 𝓘 c ψ
 
-lemma wp_weaken {𝓘 : Inv} {c : Cmd Act} {φ ψ : OProp}
-    (h : φ ⊢ ψ) : wp 𝓘 c φ ⊢ wp 𝓘 c ψ := by
-  intro 𝓟 hc μ 𝓟fr hre ν hν
-  have ⟨𝓠, hre', hφ⟩ := hc μ 𝓟fr hre ν hν
+lemma wp_conseq {𝓘 : Inv} {F : ProbSpace → Prop} {c : Cmd Act} {φ ψ : OProp}
+    (h : φ ⊢ ψ) : wp_base 𝓘 F c φ ⊢ wp_base 𝓘 F c ψ := by
+  intro 𝓟 hc μ 𝓟fr F hre ν hν
+  have ⟨𝓠, hre', hφ⟩ := hc μ 𝓟fr F hre ν hν
   refine ⟨𝓠, hre', ?_⟩; exact h 𝓠 hφ
 
-lemma wp_skip {𝓘 : Inv} (c : Cmd Act) (φ : OProp) :
-    φ ⊣⊢ wp 𝓘 Cmd.skip φ := by
+lemma wp_skip {𝓘 : Inv} {F : ProbSpace → Prop} (c : Cmd Act) (φ : OProp) :
+    φ ⊣⊢ wp_base 𝓘 F Cmd.skip φ := by
   constructor
-  · intro 𝓟 hφ μ 𝓟fr hre ν hν
+  · intro 𝓟 hφ μ 𝓟fr _ hre ν hν
     refine ⟨𝓟, ?_, hφ⟩
     rw [Cmd.withInv, Cmd.to_pom, Pom.Semantics.lin_skip, bind_pure] at hν
     obtain ⟨μ, rfl⟩ := PMF.to_distr_inv hre.bot_0
@@ -37,31 +47,31 @@ lemma wp_skip {𝓘 : Inv} (c : Cmd Act) (φ : OProp) :
     rwa [heq]
   · intro 𝓟 hφ; sorry
 
-lemma wp_seq {𝓘 : Inv} {c₁ c₂ : Cmd Act} {ψ : OProp} :
-    wp 𝓘 c₁ (wp 𝓘 c₂ ψ) ⊢ wp 𝓘 (Cmd.seq c₁ c₂) ψ := by
-  intro 𝓟 h μ 𝓟fr href ν; rw [Cmd.withInv, Cmd.to_pom, Pom.lin_seq, ← bind_assoc]
+lemma wp_seq {𝓘 : Inv} {F : ProbSpace → Prop} {c₁ c₂ : Cmd Act} {ψ : OProp} :
+    wp_base 𝓘 F c₁ (wp_base 𝓘 F c₂ ψ) ⊢ wp_base 𝓘 F (Cmd.seq c₁ c₂) ψ := by
+  intro 𝓟 h μ 𝓟fr hF href ν; rw [Cmd.withInv, Cmd.to_pom, Pom.lin_seq, ← bind_assoc]
   intro hν; rcases ConvexPowerset.mem_bind.mp hν with ⟨ξ, hξ, f, hf, rfl⟩
-  have ⟨𝓡, href', h'⟩ := h μ 𝓟fr href ξ hξ
-  refine h' ξ 𝓟fr href' _ ?_
+  have ⟨𝓡, href', h'⟩ := h μ 𝓟fr hF href ξ hξ
+  refine h' ξ 𝓟fr hF href' _ ?_
   exact ConvexPowerset.mem_bind.mpr ⟨ξ, ConvexPowerset.self_mem_singleton' _, f, hf, rfl⟩
 
-lemma wp_if_true {𝓘 : Inv} {b : Expr} {c₁ c₂ : Cmd Act} {φ ψ : OProp} :
-     ⌈b == Expr.literal 1⌉ ∧ wp 𝓘 c₁ ψ ⊢ wp 𝓘 (Cmd.if_stmt b c₁ c₂) ψ := by
-  intro 𝓟 ⟨htrue, hwp⟩ μ 𝓟fr href ν hν; rw [Cmd.withInv, Cmd.to_pom, Pom.Semantics.lin_if_stmt] at hν
+lemma wp_if_true {𝓘 : Inv} {F : ProbSpace → Prop} {b : Expr} {c₁ c₂ : Cmd Act} {φ ψ : OProp} :
+     ⌈b == Expr.literal 1⌉ ∧ wp_base 𝓘 F c₁ ψ ⊢ wp_base 𝓘 F (Cmd.if_stmt b c₁ c₂) ψ := by
+  intro 𝓟 ⟨htrue, hwp⟩ μ 𝓟fr hF href ν hν; rw [Cmd.withInv, Cmd.to_pom, Pom.Semantics.lin_if_stmt] at hν
   sorry
 
 -- This mostly follows from invariant monotonicity, but we need a few more properties about
 -- assertions, etc
-lemma wp_share {𝓘 : Inv} {c : Cmd Act} {ψ : OProp} :
-    OProp.sure 𝓘.to_MProp ∗ wp 𝓘 c ψ ⊢ wp Inv.emp c iprop(ψ ∗ OProp.sure 𝓘.to_MProp) := by
-  intro 𝓟 ⟨𝓟₁, 𝓟₂, hdisj, hle, h𝓘, hwp⟩ μ 𝓟fr hre ν hν
+lemma wp_share {𝓘 : Inv} {F : ProbSpace → Prop} {c : Cmd Act} {ψ : OProp} :
+    OProp.sure 𝓘.to_MProp ∗ wp_base 𝓘 F c ψ ⊢ wp_base Inv.emp F c iprop(ψ ∗ OProp.sure 𝓘.to_MProp) := by
+  intro 𝓟 ⟨𝓟₁, 𝓟₂, hdisj, hle, h𝓘, hwp⟩ μ 𝓟fr hF hre ν hν
   have hν' : ν ∈ ConvexPowerset.singleton' μ >>= Pom.lin (c.withInv 𝓘).to_pom := by
     refine le_iff_supset.mp ?_ hν
     apply ConvexPowerset.bind_monotone (le_refl _)
     apply (Pom.lin_continuous (act := WithInv Act) (test := Test)).monotone
     apply Cmd.withInv_monotone; refine ⟨Set.empty_subset _, ?_⟩
     intro σ; sorry
-  have ⟨𝓠, hre', hψ⟩ := hwp μ 𝓟fr sorry ν sorry
+  have ⟨𝓠, hre', hψ⟩ := hwp μ 𝓟fr hF sorry ν sorry
   refine ⟨𝓠 ⊗ ProbSpace.trivial 𝓘.to_MProp, ?_, ?_⟩
   · sorry
   · refine ⟨_, _, ?_, le_refl _, hψ, ?_⟩
@@ -70,18 +80,18 @@ lemma wp_share {𝓘 : Inv} {c : Cmd Act} {ψ : OProp} :
     · -- This should also be a lemma
       sorry
 
-lemma wp_atom {𝓘 : Inv} {a : Act} {ψ : OProp} :
-    (OProp.sure 𝓘.to_MProp -∗ wp Inv.emp (Cmd.act a) (iprop(ψ ∗ OProp.sure 𝓘.to_MProp)))
-    ⊢ wp 𝓘 (Cmd.act a) ψ := by
+lemma wp_atom {𝓘 : Inv} {F : ProbSpace → Prop} {a : Act} {ψ : OProp} :
+    (OProp.sure 𝓘.to_MProp -∗ wp_base Inv.emp F (Cmd.act a) (iprop(ψ ∗ OProp.sure 𝓘.to_MProp)))
+    ⊢ wp_base 𝓘 F (Cmd.act a) ψ := by
   sorry
 
-lemma wp_assign {𝓘 : Inv} (x : Var) (e : Expr) (ψ : OProp) (v : Val) :
+lemma wp_assign {𝓘 : Inv} {F : ProbSpace → Prop} (x : Var) (e : Expr) (ψ : OProp) (v : Val) :
   (OProp.sure ($ x == Expr.literal v) ∗ (OProp.sure ($ x == (fun σ ↦ e (σ.extend x v))) -∗ ψ)) ⊢
-  wp 𝓘 (x ::= e) ψ := sorry
+  wp_base 𝓘 F (x ::= e) ψ := sorry
 
-lemma wp_assign' {𝓘 : Inv} (x : Var) (e : Expr) {ψ : OProp} :
+lemma wp_assign' {𝓘 : Inv} {F : ProbSpace → Prop} (x : Var) (e : Expr) {ψ : OProp} :
   (OProp.sure (MProp.own ($ x))) ∗ (OProp.sure ($ x == e) -∗ ψ) ⊢
-  wp 𝓘 (x ::= e) ψ := sorry
+  wp_base 𝓘 F (x ::= e) ψ := sorry
 
 /-- **The parallel composition rule.**  If the postconditions `ψ₁` and `ψ₂` are precise, then
 the weakest preconditions of two threads can be combined with the separating conjunction.
@@ -93,7 +103,7 @@ of `𝓠ₖ`, and the two threads are then combined by `lemma_C6`. -/
 lemma wp_par {𝓘 : Inv} {c₁ c₂ : Cmd Act} {ψ₁ ψ₂ : OProp}
     (hψ₁ : ψ₁.Precise) (hψ₂ : ψ₂.Precise) :
     wp 𝓘 c₁ ψ₁ ∗ wp 𝓘 c₂ ψ₂ ⊢ wp 𝓘 (c₁.par c₂) iprop(ψ₁ ∗ ψ₂) := by
-  intro 𝓟 ⟨𝓟₁, 𝓟₂, hdisj, hle, h₁, h₂⟩ μ 𝓟fr hre ν hν
+  intro 𝓟 ⟨𝓟₁, 𝓟₂, hdisj, hle, h₁, h₂⟩ μ 𝓟fr _ hre ν hν
   -- `𝓠₁` and `𝓠₂` are the least probability spaces satisfying `ψ₁` and `ψ₂`
   obtain ⟨𝓠₁, hQ₁⟩ := hψ₁
   obtain ⟨𝓠₂, hQ₂⟩ := hψ₂
@@ -112,7 +122,7 @@ lemma wp_par {𝓘 : Inv} {c₁ c₂ : Cmd Act} {ψ₁ ψ₂ : OProp}
       ∀ ν₁ ∈ ConvexPowerset.singleton' μ₁ >>= 𝓛 (c₁.withInv 𝓘).to_pom,
         ((𝓠₁ ⊗ 𝓕 ⊗ ProbSpace.trivial 𝓘.to_MProp) ≼ ν₁) := by
     intro 𝓕 μ₁ hre₁ ν₁ hν₁
-    obtain ⟨𝓠, href, hψ⟩ := h₁ μ₁ 𝓕 hre₁ ν₁ hν₁
+    obtain ⟨𝓠, href, hψ⟩ := h₁ μ₁ 𝓕 True.intro hre₁ ν₁ hν₁
     exact Distr.Refines.mono
       (ProbSpace.product_mono_left (ProbSpace.product_mono_left ((hQ₁ 𝓠).mpr hψ))) href
   have hthread₂ : ∀ (𝓕 : ProbSpace) (μ₂ : Distr Mem),
@@ -120,16 +130,16 @@ lemma wp_par {𝓘 : Inv} {c₁ c₂ : Cmd Act} {ψ₁ ψ₂ : OProp}
       ∀ ν₂ ∈ ConvexPowerset.singleton' μ₂ >>= 𝓛 (c₂.withInv 𝓘).to_pom,
         ((𝓠₂ ⊗ 𝓕 ⊗ ProbSpace.trivial 𝓘.to_MProp) ≼ ν₂) := by
     intro 𝓕 μ₂ hre₂ ν₂ hν₂
-    obtain ⟨𝓠, href, hψ⟩ := h₂ μ₂ 𝓕 hre₂ ν₂ hν₂
+    obtain ⟨𝓠, href, hψ⟩ := h₂ μ₂ 𝓕 True.intro hre₂ ν₂ hν₂
     exact Distr.Refines.mono
       (ProbSpace.product_mono_left (ProbSpace.product_mono_left ((hQ₂ 𝓠).mpr hψ))) href
   -- The parallel composition is handled by Lemma C.6
   rw [Cmd.withInv, Cmd.to_pom] at hν
   exact lemma_C6 hμ hthread₁ hthread₂ ν hν
 
-lemma wp_split {𝓘 : Inv} {c : Cmd Act} {ξ : PMF Val} {ψ : Val → OProp} :
-    (⨁[ ξ ] fun v ↦ wp 𝓘 c (ψ v)) ⊢ wp 𝓘 c (⨁[ ξ ] ψ) := by
-  intro 𝓟 ⟨𝓟', V, hdsj, hdom, hsum, hwp⟩ μ 𝓟fr hre ν hν
+lemma wp_split {𝓘 : Inv} {F : ProbSpace → Prop} {c : Cmd Act} {ξ : PMF Val} {ψ : Val → OProp} :
+    (⨁[ ξ ] fun v ↦ wp_base 𝓘 F c (ψ v)) ⊢ wp_base 𝓘 F c (⨁[ ξ ] ψ) := by
+  intro 𝓟 ⟨𝓟', V, hdsj, hdom, hsum, hwp⟩ μ 𝓟fr hF hre ν hν
   obtain ⟨k, rfl, hk⟩ :
       ∃ k,
         μ = ξ.bind k ∧
@@ -137,7 +147,7 @@ lemma wp_split {𝓘 : Inv} {c : Cmd Act} {ξ : PMF Val} {ψ : Val → OProp} :
     sorry
   obtain ⟨ξ', _, f, hf, rfl⟩ := ConvexPowerset.mem_bind.mp hν
   have : ξ' = ξ.bind k := sorry; subst this
-  have h v hv := hwp v hv (k v) 𝓟fr (hk v hv) ((k v).bind f) sorry
+  have h v hv := hwp v hv (k v) 𝓟fr hF (hk v hv) ((k v).bind f) sorry
   choose 𝓠 h𝓠 using h
   classical
   let 𝓠' v := if h : v ∈ ξ.support then 𝓠 v h else ProbSpace.trivial Iris.BI.BIBase.emp
@@ -147,5 +157,14 @@ lemma wp_split {𝓘 : Inv} {c : Cmd Act} {ξ : PMF Val} {ψ : Val → OProp} :
   · refine ⟨𝓠', V, sorry, sorry, le_refl _, ?_⟩
     intro v hv; unfold 𝓠'; rw [dif_pos hv]
     exact h𝓠 v hv |>.2
+
+lemma wp_weaken {𝓘 : Inv} {c : Cmd Act} {ψ : OProp} :
+    wp 𝓘 c ψ ⊢ wp_weak 𝓘 c ψ := by
+  intro 𝓟 hwp μ 𝓕 _ hre ν hν
+  exact hwp μ 𝓕 True.intro hre ν hν
+
+lemma wp_strengthen {𝓘 : Inv} {c : Cmd Act} {ψ : OProp} (h : ψ.Precise) :
+    wp_weak 𝓘 c ψ ⊢ wp 𝓘 c ψ := by
+  sorry
 
 end Pcol
